Incorrectness definition name is updated. Assign, If, Seq rules are added.

Incorrectness/Defs.lean
@@ -3,7 +3,7 @@ open Language
 namespace Incorrectness
 
 -- [P] S [Q] : Under-approximation
-def IncorrectnessHoare (P : State → Prop)
+def Incorrectness (P : State → Prop)
         (S : Stmt)
         (Q : State → Prop) : Prop :=
   ∀ t, Q t → ∃ s, P s ∧ (S, s) ⟹ t
@@ -12,6 +12,6 @@ def IncorrectnessHoare (P : State → Prop)
 -- Syntactic Sugar
 -- Allows writing [* P *] (S) [* Q *]
 notation "[* " P " *] " "(" S ")" " [* " Q " *]"
-  => IncorrectnessHoare P S Q
+  => Incorrectness P S Q
 
 end Incorrectness
