Incorrectness/Assign.lean
@@ -1,0 +1,34 @@
+import Incorrectness.Defs
+open Language
+namespace Incorrectness
+
+-- The Assignment Rule
+-- Q = { t | ∃ s, P s ∧ t = s[x ↦ a s] }
+--
+theorem assign_intro {P : State → Prop}
+    {x : String}
+    {a : State → Nat} :
+  [* P *] (Stmt.assign x a) [* fun t => ∃ s, P s ∧ t = (s[x ↦ a s]) *] :=
+  by
+  -- Introduction
+  -- t: final state
+  -- h_post: hypothesis (Postcondition holds for the final state)
+  intro t h_post
+
+  cases h_post with
+      -- s_prev : The previous state
+      -- h_and  : hypothesis (P holds for s_prev ∧ t = s_prev[x ↦ a s_prev])
+    | intro s_prev h_and =>
+      cases h_and with
+        -- hP     : P holds for s_prev
+        -- hEq    : t is indeed s_prev updated with x assigned to (a s_prev)
+      | intro hP hEq =>
+        exists s_prev
+
+        apply And.intro
+        exact hP
+
+        rw [hEq]
+        exact BigStep.assign x a s_prev
+
+end Incorrectness
