Incorrectness/If.lean
@@ -1,0 +1,65 @@
+import Incorrectness.Defs
+open Language
+namespace Incorrectness
+
+-- The Conditional Rule (If-Then-Else)
+--
+--        [P ∧ B] S [Q]    [P ∧ ¬B] T [Q]
+-- -------------------------------------------
+--        [P] if B then S else T [Q]
+
+theorem if_intro {P Q1 Q2 : State → Prop}
+    {B : State → Prop}
+    {S1 S2 : Stmt}
+  (h1 : [* fun s => P s ∧ B s *] (S1) [* Q1 *])
+  (h2 : [* fun s => P s ∧ ¬B s *] (S2) [* Q2 *]) :
+  [* P *] (Stmt.ifThenElse B S1 S2) [* fun t => Q1 t ∨ Q2 t *] :=
+  by
+  -- Introduce variables and hypotheses
+  -- t: final state
+  -- h_post: hypothesis that the postcondition holds in state t
+  intro t h_post
+
+  cases h_post with
+  -- CASE 1: The TRUE Branch (S1 executed)
+  | inl hQ1 =>
+    -- Use hypothesis h1 to find the start state 's'
+    -- h1 says: If we are in Q1, we came from 's' where (P s ∧ B s).
+    have h1_unfolded := h1 t hQ1
+    cases h1_unfolded with
+    -- s : The initial state
+    -- h_start : (P s ∧ B s) and (S1, s) executes to t
+    | intro s h_start =>
+      cases h_start with
+      -- hPre1  : (P s ∧ B s)
+      -- hExec1 : (S1, s) executes to t
+      | intro hPre1 hExec1 =>
+        exists s
+        apply And.intro
+        exact hPre1.left
+
+        apply BigStep.if_true B S1 S2 s t
+        exact hPre1.right -- Proof that condition B is true
+        exact hExec1      -- Proof that S1 executes to t
+
+  -- CASE 2: The FALSE Branch (S2 executed)
+  | inr hQ2 =>
+    -- Use hypothesis h2 to find the start state 's'
+    -- h2 says: If we are in Q2, we came from 's' where (P s ∧ ¬B s).
+    have h2_unfolded := h2 t hQ2
+    cases h2_unfolded with
+    -- s : The initial state
+    -- h_start : (P s ∧ ¬B s) and (S2, s) executes to t
+    | intro s h_start =>
+      cases h_start with
+      -- hPre2  : (P s ∧ ¬B s)
+      -- hExec2 : (S2, s) executes to t
+      | intro hPre2 hExec2 =>
+        exists s
+        apply And.intro
+        exact hPre2.left
+
+        apply BigStep.if_false B S1 S2 s t
+        exact hPre2.right -- Proof that condition B is false (¬B)
+        exact hExec2      -- Proof that S2 executes to t
+end Incorrectness
