Incorrectness/Seq.lean
@@ -1,0 +1,46 @@
+import Incorrectness.Defs
+open Language
+namespace Incorrectness
+
+-- The Sequence Rule
+-- [P] S [Q]   [Q] T [R]
+-- ---------------------
+--     [P] S; T [R]
+--
+-- This is standard composition: [P] S1 [Q] and [Q] S2 [R] implies [P] S1;S2 [R]
+--
+theorem seq_intro {P Q R : State → Prop} {S1 S2 : Stmt}
+  (h1 : [* P *] (S1) [* Q *])
+  (h2 : [* Q *] (S2) [* R *]) :
+  [* P *] (S1; S2) [* R *] :=
+  by
+  -- Introduce variables and hypotheses
+  -- t: final state
+  -- hR: hypothesis that R holds in state t (Postcondition)
+  intro t hR
+
+  have h2_unfolded := h2 t hR
+  cases h2_unfolded with
+  -- s2 : The intermediate state
+  -- h_intermediate : Q holds at s2 ∧ (S2, s2) executes to t
+  | intro s2 h_intermediate =>
+    cases h_intermediate with
+  -- hQ     : Q holds at s2
+  -- hExec2 : (S2, s2) executes to t
+    | intro hQ hExec2 =>
+      have h1_unfolded := h1 s2 hQ
+      cases h1_unfolded with
+      -- s1 : The initial state
+      -- h_start : P holds at s1 ∧ (S1, s1) executes to s2
+      | intro s1 h_start =>
+        cases h_start with
+      -- hP     : P holds at s1
+      -- hExec1 : (S1, s1) executes to s2
+        | intro hP hExec1 =>
+        exists s1
+
+        apply And.intro
+        exact hP
+        exact BigStep.seq S1 S2 s1 s2 t hExec1 hExec2
+
+end Incorrectness
